code/tests/Hacl.Test.ECDSA.fst
@@ -298,7 +298,7 @@ let test_siggen_256 (vec:siggen_vector) : Stack unit (requires fun _ -> True) (e
     B.blit qx 0ul qxy 0ul 32ul;
     B.blit qy 0ul qxy 32ul 32ul; 
 
-    let flag = ecdsa_sign_p256_sha2 rs msg_len msg d k in 
+    let flag = ecdsa_sign_p256_sha2_def rs msg_len msg d k in 
     if Lib.RawIntTypes.u64_to_UInt64 flag = 0uL then
       begin
       let okr = compare_and_print (B.sub rs 0ul 32ul) r 32ul in 
