code/ecdsap256/Hacl.Impl.P256.ECDSA.Defensive.fst
@@ -1,0 +1,72 @@
+module Hacl.Impl.P256.ECDSA.Defensive
+
+open FStar.HyperStack.All
+open FStar.HyperStack
+module ST = FStar.HyperStack.ST
+
+open Lib.IntTypes
+open Lib.Buffer
+open Lib.ByteSequence
+
+open Spec.ECDSA
+open Spec.P256.Lemmas
+
+open FStar.Mul
+open FStar.Math.Lemmas
+
+open Hacl.Hash.SHA2
+
+open Spec.P256
+open Spec.P256.Lemmas
+open Spec.P256.Definitions
+
+open Spec.ECDSAP256.Definition
+
+open Hacl.Impl.P256.LowLevel 
+
+open Hacl.Impl.P256.Core
+
+open Hacl.Impl.ECDSA.MM.Exponent
+open Hacl.Impl.ECDSA.MontgomeryMultiplication
+
+open Hacl.Impl.P256.Signature.Common
+
+module H = Spec.Agile.Hash
+module Def = Spec.Hash.Definitions
+
+open Spec.Hash.Definitions
+
+open Hacl.Impl.ECDSA.P256.Signature.Agile
+
+
+
+inline_for_extraction noextract
+val ecdsa_sign_p256_sha2_def: alg: hash_alg_ecdsa 
+  -> result: lbuffer uint8 (size 64) 
+  -> mLen: size_t {v mLen >= Spec.ECDSA.min_input_length alg}
+  -> m: lbuffer uint8 mLen 
+  -> privKey: lbuffer uint8 (size 32) 
+  -> k: lbuffer uint8 (size 32) -> 
+  Stack uint64
+  (requires fun h -> 
+    live h result /\ live h m /\ live h privKey /\ live h k /\
+    disjoint result m /\
+    disjoint result privKey /\
+    disjoint result k /\
+    nat_from_bytes_be (as_seq h privKey) < prime_p256_order /\
+    nat_from_bytes_be (as_seq h k) < prime_p256_order
+  )
+  (ensures fun h0 flag h1 -> 
+    modifies (loc result) h0 h1 /\
+     (assert_norm (pow2 32 < pow2 61);
+      let resultR = gsub result (size 0) (size 32) in 
+      let resultS = gsub result (size 32) (size 32) in 
+      let r, s, flagSpec = Spec.ECDSA.ecdsa_signature_agile alg (uint_v mLen) (as_seq h0 m) (as_seq h0 privKey) (as_seq h0 k) in 
+      as_seq h1 resultR == nat_to_bytes_be 32 r /\
+      as_seq h1 resultS == nat_to_bytes_be 32 s /\
+      flag == flagSpec 
+    )    
+  )
+
+
+let ecdsa_sign_p256_sha2_def alg result mLen m privKey k = ecdsa_signature alg result mLen m privKey k
