code/ecdsap256/Hacl.P256.fsti
@@ -402,3 +402,51 @@ val ecp256dh_r:
       as_seq h1 (gsub result (size 32) (size 32)) == pointY)
 
 
+
+
+
+
+
+
+
+
+
+
+
+
+
+
+
+
+
+
+
+[@ (Comment " Input: result buffer: uint8[64], \n m buffer: uint8 [mLen], \n priv(ate)Key: uint8[32], \n k (nonce): uint32[32]. 
+  \n Output: uint64, where 0 stands for the correct signature generation. All the other values mean that an error has occurred. 
+  \n The private key and the nonce are expected to be less than the curve order.")]
+
+val ecdsa_sign_p256_sha2_def: result: lbuffer uint8 (size 64) 
+  -> mLen: size_t 
+  -> m: lbuffer uint8 mLen 
+  -> privKey: lbuffer uint8 (size 32) 
+  -> k: lbuffer uint8 (size 32) -> 
+  Stack uint64
+  (requires fun h -> 
+    live h result /\ live h m /\ live h privKey /\ live h k /\
+    disjoint result m /\
+    disjoint result privKey /\
+    disjoint result k /\
+    nat_from_bytes_be (as_seq h privKey) < prime_p256_order /\
+    nat_from_bytes_be (as_seq h k) < prime_p256_order
+  )
+  (ensures fun h0 flag h1 -> 
+    modifies (loc result) h0 h1 /\
+     (assert_norm (pow2 32 < pow2 61);
+      let resultR = gsub result (size 0) (size 32) in 
+      let resultS = gsub result (size 32) (size 32) in 
+      let r, s, flagSpec = Spec.ECDSA.ecdsa_signature_agile (Spec.ECDSA.Hash SHA2_256) (uint_v mLen) (as_seq h0 m) (as_seq h0 privKey) (as_seq h0 k) in 
+      as_seq h1 resultR == nat_to_bytes_be 32 r /\
+      as_seq h1 resultS == nat_to_bytes_be 32 s /\
+      flag == flagSpec 
+    )    
+  )
